HMAC circuit update (#901)
Working HMAC circuit - we can set the key registers and stream data to the fifo and it produces the correct value in the digest registers.

silveroak-opentitan/hmac/hw/Hmac.v
@@ -21,6 +21,7 @@ Require Import Cava.Types.
 Require Import Cava.Expr.
 Require Import Cava.Primitives.
 Require Import Cava.TLUL.
+Require Import Cava.Fifo.
 
 Require Import HmacHardware.Sha256.
 Import ExprNotations.
@@ -33,11 +34,147 @@ Section Var.
   Context {var : tvar}.
 
   Definition hmac_register_count := 27%nat.
-  Definition hmac_register_index := 5%nat.
-  Definition hmac_register := BitVec hmac_register_index.
+  Definition hmac_register_log_sz := 5%nat.
 
-  Definition REG_INTR_STATE := Constant hmac_register 0.
-  Definition REG_CMD := Constant hmac_register 5.
+  Definition REG_INTR_STATE := Constant (BitVec hmac_register_log_sz) 0.
+  Definition REG_CMD := Constant (BitVec hmac_register_log_sz) 5.
+  Definition REG_INTR := Constant (BitVec hmac_register_log_sz) 0.
+  Definition REG_DIGEST_0 := Constant (BitVec hmac_register_log_sz) 0x11.
+  Definition REG_DIGEST_1 := Constant (BitVec hmac_register_log_sz) 0x12.
+  Definition REG_DIGEST_2 := Constant (BitVec hmac_register_log_sz) 0x13.
+  Definition REG_DIGEST_3 := Constant (BitVec hmac_register_log_sz) 0x14.
+  Definition REG_DIGEST_4 := Constant (BitVec hmac_register_log_sz) 0x15.
+  Definition REG_DIGEST_5 := Constant (BitVec hmac_register_log_sz) 0x16.
+  Definition REG_DIGEST_6 := Constant (BitVec hmac_register_log_sz) 0x17.
+  Definition REG_DIGEST_7 := Constant (BitVec hmac_register_log_sz) 0x18.
+  Definition REG_KEY_0 := Constant (BitVec hmac_register_log_sz) 0x9.
+  Definition REG_KEY_1 := Constant (BitVec hmac_register_log_sz) 0xA.
+  Definition REG_KEY_2 := Constant (BitVec hmac_register_log_sz) 0xB.
+  Definition REG_KEY_3 := Constant (BitVec hmac_register_log_sz) 0xC.
+  Definition REG_KEY_4 := Constant (BitVec hmac_register_log_sz) 0xD.
+  Definition REG_KEY_5 := Constant (BitVec hmac_register_log_sz) 0xE.
+  Definition REG_KEY_6 := Constant (BitVec hmac_register_log_sz) 0xF.
+  Definition REG_KEY_7 := Constant (BitVec hmac_register_log_sz) 0x10.
+
+  (* Hmac_inner uses realigned fifo values and regsiter map *)
+  (* state value = *)
+  (* 1. Hash key ^ ipad *)
+  (* 2. Hash message *)
+  (* 3. Store digest and reset sha256 *)
+  (* 4. Hash key ^ opad *)
+  (* 5. Hash stored digest *)
+  (* 6. Store digest and reset sha256 *)
+  Definition hmac_inner : Circuit _
+    [Vec (BitVec 32) hmac_register_count; Bit; BitVec 32; BitVec 4; Bit]
+    (Vec (BitVec 32) hmac_register_count ** Bit) := {{
+    fun registers fifo_valid fifo_data fifo_length fifo_final =>
+
+    let/delay '(updated_registers, waiting_for_digest, accept_fifo, ptr, state, digest; sha_ready) :=
+
+      let cmd_hash_start   := (`index` registers `REG_CMD` & `K 0x1`) == `K 0x1` in
+      let cmd_hash_process := (`index` registers `REG_CMD` & `K 0x2`) == `K 0x2` in
+
+      let state' : BitVec 5 :=
+             if sha_ready && state == `K 1` && ptr == `K 15` then state + `K 1`
+        (* cmd_hash_process is the end of message, but we also have to wait for
+         * fifo to drain by observing fifo_valid *)
+        else if sha_ready && state == `K 2` && cmd_hash_process && !fifo_valid  then state + `K 1`
+        else if             state == `K 3`  && (!waiting_for_digest) then state + `K 1`
+        else if sha_ready && state == `K 4` && ptr == `K 15` then state + `K 1`
+        else if sha_ready && state == `K 5` && ptr == `K 7`  then state + `K 1`
+        else if sha_ready && state == `K 6` && (!waiting_for_digest) then `K 0`
+        else if state == `K 0` && cmd_hash_start then `K 1`
+        else state in
+
+      let ptr' : BitVec 6 :=
+             if (state == `K 0`) || ! (state == state') then `K 0`
+        else if !sha_ready then ptr
+        else (ptr + `K 1`) in
+
+      (* Keys start at byte address 0x24 or the 9th 32bit register *)
+      let key_vec := `slice 9 8` registers in
+      let key := `index` key_vec ptr in
+      let digest_word := `index` digest ptr in
+
+      let '(sha_stream_valid, sha_stream, sha_stream_final; sha_stream_final_length) :=
+             if state == `K 1` then (`True`, key ^ `K 0x36363636`, `False`, `K 0`)
+        else if state == `K 2` then (fifo_valid, fifo_data, fifo_final, fifo_length)
+        (* else if state' == `K 3` *)
+        else if state == `K 4` then (`True`, key ^ `K 0x5c5c5c5c`, `False`, `K 0`)
+        else if state == `K 5` then (`True`, digest_word, (ptr == `K 7` ) , `K 4`)
+        else (`False`, `K 0`, `False`, `K 0`)
+
+      in
+
+      (* I don't think we need to explicitly flush-
+         if we are left in a bad state we might need to flush after the last state
+      *)
+      let sha_stream_flush := `False` in
+
+      let '(sha_done, sha_digest; sha_ready)
+        := `sha256` sha_stream_valid sha_stream sha_stream_final sha_stream_final_length sha_stream_flush in
+
+      let is_consuming := state' == `K 2` && sha_ready in
+      let next_digest := if sha_done then sha_digest else digest in
+
+      (* update registers, alternatively this could moved outside hmac_inner *)
+      let next_registers :=
+        (* assert the INTR register `hmac_done` when we finish *)
+        (fun regs => if (state == `K 6`) && (state' == `K 0`) then
+          let regs := `replace` regs `REG_INTR` `K 1` in
+          let regs := `replace` regs `REG_DIGEST_0` ( `index` sha_digest `Constant (BitVec 4) 0` ) in
+          let regs := `replace` regs `REG_DIGEST_1` ( `index` sha_digest `Constant (BitVec 4) 1` ) in
+          let regs := `replace` regs `REG_DIGEST_2` ( `index` sha_digest `Constant (BitVec 4) 2` ) in
+          let regs := `replace` regs `REG_DIGEST_3` ( `index` sha_digest `Constant (BitVec 4) 3` ) in
+          let regs := `replace` regs `REG_DIGEST_4` ( `index` sha_digest `Constant (BitVec 4) 4` ) in
+          let regs := `replace` regs `REG_DIGEST_5` ( `index` sha_digest `Constant (BitVec 4) 5` ) in
+          let regs := `replace` regs `REG_DIGEST_6` ( `index` sha_digest `Constant (BitVec 4) 6` ) in
+          let regs := `replace` regs `REG_DIGEST_7` ( `index` sha_digest `Constant (BitVec 4) 7` ) in
+          regs
+        else regs)
+        (* deassert the CMD registers once we no longer need them @ state > 3 *)
+        (if state == `K 3` then `replace` registers `REG_CMD` `K 0` else registers)
+      in
+
+      let waiting_for_digest :=
+        if (state' == `K 3`) || (state' == `K 6`)
+        then ! sha_done
+        else `False` in
+
+      (next_registers, waiting_for_digest, is_consuming, ptr', state', next_digest, sha_ready)
+
+      initially default
+    in
+
+    (updated_registers, accept_fifo)
+
+  }}.
+
+  Definition hmac : Circuit _ [Bit; BitVec 32; BitVec 5; BitVec 4; Bit] (Vec (BitVec 32) hmac_register_count) := {{
+    fun write_en write_data write_address write_mask is_fifo_write =>
+    let/delay '(sha_ready ; registers) :=
+
+      (* TODO(blaxill): mask RO register writes *)
+      let next_registers :=
+        if write_en && !is_fifo_write
+        then `replace (n:=hmac_register_count)` registers write_address write_data
+        else registers
+      in
+
+      let cmd_hash_process := (`index` registers `REG_CMD` & `K 0x2`) == `K 0x2` in
+
+      let '(fifo_valid, fifo_data, fifo_data_length, fifo_is_last; fifo_full) :=
+        `realign_fifo 256` (write_en && is_fifo_write) write_data write_mask cmd_hash_process sha_ready in
+
+      let '(registers'; sha_ready) :=
+        `hmac_inner` next_registers fifo_valid fifo_data fifo_data_length fifo_is_last in
+
+      (sha_ready, registers')
+      initially default
+
+    in (registers)
+  }}.
+
 
   Definition hmac_top : Circuit _ [tl_h2d_t] tl_d2h_t := {{
     fun incoming_tlp =>
@@ -46,39 +183,110 @@ Section Var.
 
       let '(tl_o, write_en, write_address, write_data; write_mask)
         := `tlul_adapter_reg` incoming_tlp registers in
+
       let aligned_address := `bvslice 2 5` write_address in
 
-      let fifo_write := write_address >= `Constant (BitVec _) 2048` in
+      let is_fifo_write := write_address >= `Constant (BitVec _) 2048` in
 
-      (* TODO(blaxill): ignore/mask writes to CMD etc ? *)
-      (* TODO(blaxill): apply mask to register writes*)
-      let nregisters :=
-        if write_en && !fifo_write
-        then `replace (n:=hmac_register_count)` registers aligned_address write_data
-        else registers
-      in
+      let registers' := `hmac` write_en write_data aligned_address write_mask is_fifo_write in
 
-      (* cmd_start is set when host writes to hmac.CMD.hash_start *)
-      (* and signifies the start of a new message *)
-      let cmd_start := write_en && aligned_address == `REG_CMD` && write_data == `K 1` && !fifo_write in
-      (* cmd_process is set when host writes to hmac.CMD.hash_process *)
-      (* and signifies the end of a message *)
-      let cmd_process := write_en && aligned_address == `REG_CMD` && write_data == `K 2` && !fifo_write in
+      (tl_o, registers')
 
-      let '(packer_valid; packer_data)
-        := `tlul_pack` (write_en && fifo_write) write_data write_mask cmd_process in
-
-      (* TODO(blaxill): FIX ME *)
-      (* let '(_, padded_block; padded_valid) := `sha256_padder` packer_valid packer_data cmd_process `circuit_hole` cmd_start in *)
-      (* TODO(blaxill): sha needs to block FIFO writes and process HMAC key first *)
-      (* let inital_digest := `Constant _ sha256_initial_digest` in *)
-      (* let '(digest; digest_valid) := `sha256_inner` padded_block padded_valid `circuit_hole` in *)
-      (* let next_digest := if digest_valid then digest else digest_buffer in *)
-
-      (tl_o, nregisters)
-
-      initially value_hole
+      initially default
     in tl_o
   }}.
 
 End Var.
+
+Section SanityCheck.
+  Require Import Cava.Semantics.
+  Require Import Coq.Lists.List.
+  Import ListNotations.
+  Open Scope list_scope.
+  Close Scope circuit_type_scope.
+
+  Definition pp {n} (v: denote_type (Vec (BitVec 32) n)) :=
+    List.map HexString.of_N v.
+
+  Definition is_done (v : denote_type (Vec (BitVec 32) hmac_register_count)) :=
+    nth 0 (v) 0.
+
+  Definition state_of {s i o} (_: Circuit (var:=denote_type) s i o) := s.
+
+  Definition get_regs (v: denote_type (state_of hmac))
+    : denote_type (Vec (BitVec 32) hmac_register_count) .
+    cbv [state_of hmac absorb_any] in v.
+    destruct v.
+    destruct d as (_, regs).
+    exact regs.
+  Defined.
+
+  (* We can set registers *)
+  Goal
+    let write_en := true in
+    let write_data := 0xAAAAAAAAA in
+    let write_address := 26 in
+    let write_mask := 0xFFFFFFFF in
+    let is_fifo_write := false in
+    forall write_data,
+    nth (N.to_nat write_address) (get_regs (
+      fst (step hmac
+         (reset_state hmac)
+         (write_en, (write_data, (write_address, (write_mask, (is_fifo_write, tt)))))
+      ))) 0
+    = write_data.
+  Proof. vm_compute; reflexivity. Qed.
+
+  (* Set the key registers to the test key *)
+  Definition state_with_key_registers_set :=
+    Eval vm_compute in
+    snd (simulate' hmac (
+     List.map (fun v => (true, (snd v, (9 + fst v, (0xF, (false, tt))))))
+      [ (0, 0x00010203)
+      ; (1, 0x04050607)
+      ; (2, 0x08090A0B)
+      ; (3, 0x0C0D0E0F)
+      ; (4, 0x10111213)
+      ; (5, 0x14151617)
+      ; (6, 0x18191A1B)
+      ; (7, 0x1C1D1E1F)
+      ]) (reset_state hmac)).
+
+  (* digest registers get set to the correct digest *)
+  Goal
+    (* there are 8 digest registers start at 0x11*)
+    firstn 8 (skipn 0x11
+    (get_regs (snd (
+    simulate' hmac
+    (
+     (* set cmd_start *)
+     [ (true, (1, (5, (0xF, (false, tt))))) ] ++
+
+     (* send message data to fifo *)
+     (
+     List.map (fun v => (true, (snd v, (512, (fst v, (true, tt))))))
+      [
+      ( 0xF, 0x53616D70 )
+    ; ( 0xF, 0x6C65206D )
+    ; ( 0xF, 0x65737361 )
+    ; ( 0xF, 0x67652066 )
+    ; ( 0xF, 0x6F72206B )
+    ; ( 0xF, 0x65796C65 )
+    ; ( 0xF, 0x6E3C626C )
+    ; ( 0xF, 0x6F636B6C )
+    ; ( 0xC, 0x656E0000 )
+
+      ])
+
+     (* signal cmd_processm  *)
+      ++ [ (true, (3, (5, (0xF, (false, tt))))) ]
+
+     (* wait for digest to be ready *)
+     ++ repeat (false, (0, (0, (0, (false, tt))))) 350
+      )
+      state_with_key_registers_set))))
+    = [0xA28CF431; 0x30EE696A; 0x98F14A37; 0x678B56BC; 0xFCBDD9E5; 0xCF69717F; 0xECF5480F; 0x0EBDF790].
+
+  Proof. Time vm_compute; reflexivity. Qed.
+
+End SanityCheck.
